SlaneyRLScript.sml
@@ -16,10 +16,10 @@ End
 val _ = set_fixity "-->ₛ" (Infixr 490);
 val _ = overload_on ("-->ₛ", “s_IMP”);
 
-val _ = set_fixity "&ₛ" (Infixr 490); 
+val _ = set_fixity "&ₛ" (Infixl 600); 
 val _ = overload_on ("&ₛ", “s_AND”);
 
-val _ = set_fixity "Vₛ" (Infixr 490);
+val _ = set_fixity "Vₛ" (Infixl 500);
 val _ = overload_on ("Vₛ", “s_OR”);
 
 val _ = overload_on ("~ₛ", “s_NOT”);
@@ -31,10 +31,10 @@ Definition s_DIMP_def:
 End
 
     
-val _ = set_fixity "<->ₛ" (Infixr 490);
+val _ = set_fixity "<->ₛ" (Infixr 491);
 val _ = overload_on ("<->ₛ", “s_DIMP”);
  
-val _ = set_fixity "ioₛ" (Infixr 490);
+val _ = set_fixity "ioₛ" (Infixl 600);
 val _ = overload_on ("ioₛ", “s_ICONJ”);
                 
 Inductive slaney_provable: 
@@ -90,49 +90,50 @@ Theorem s_equiv_transitivity:
 Proof
   metis_tac[s_adjunction_rule, s_transitivity, s_conjunction_l, s_conjunction_r, s_conj_introduction, s_DIMP_def, s_modus_ponens] 
 QED
+
+Theorem s_conj_intro_rule:
+  ∀A B C. slaney_provable (A -->ₛ B) ∧
+          slaney_provable (A -->ₛ C) ⇒
+          slaney_provable (A -->ₛ (B &ₛ C))
+Proof
+  metis_tac[slaney_provable_rules]
+QED
         
 Theorem s_equiv_replacement:
   ∀A B C. slaney_provable (A <->ₛ B) ⇒
-          (slaney_provable (A -->ₛ C) ⇔ slaney_provable (B -->ₛ C)) ∧
-          (slaney_provable (C -->ₛ A) ⇔ slaney_provable (C -->ₛ B)) ∧
-          (slaney_provable (A &ₛ C) ⇔ slaney_provable (B &ₛ C)) ∧
-          (slaney_provable (C &ₛ A) ⇔ slaney_provable (C &ₛ A)) ∧
-          (slaney_provable (A Vₛ C) ⇔ slaney_provable (B Vₛ C)) ∧
-          (slaney_provable (C Vₛ A) ⇔ slaney_provable (C Vₛ A)) ∧
+          (slaney_provable ((A -->ₛ C) <->ₛ (B -->ₛ C))) ∧
+          (slaney_provable ((C -->ₛ A) <->ₛ (C -->ₛ B))) ∧
+          slaney_provable (~ₛ A <->ₛ ~ₛ B) ∧ 
+          (slaney_provable ((A &ₛ C) <->ₛ (B &ₛ C))) ∧
+          (slaney_provable ((C &ₛ A) <->ₛ (C &ₛ A))) ∧
+          (slaney_provable ((A Vₛ C) <->ₛ (B Vₛ C))) ∧
+          (slaney_provable ((C Vₛ A) <->ₛ (C Vₛ A))) ∧
+          (slaney_provable ((A ioₛ C) <->ₛ (B ioₛ C))) ∧
+          (slaney_provable ((C ioₛ A) <->ₛ (C ioₛ A))) ∧
+          (slaney_provable ((A <->ₛ C) <->ₛ (B <->ₛ C))) ∧
+          (slaney_provable ((C <->ₛ A) <->ₛ (C <->ₛ A))) ∧                
           (slaney_provable (A) ⇔ slaney_provable (B))
 Proof
-  rpt strip_tac >> EQ_TAC >> gs [s_DIMP_def]
-  >- metis_tac [s_conjunction_r, s_conjunction_l, s_transitivity, s_modus_ponens, s_adjunction_rule]
-  >- metis_tac [s_conjunction_r, s_conjunction_l, s_transitivity, s_modus_ponens, s_adjunction_rule]                          
-  >- metis_tac [s_conjunction_r, s_conjunction_l, s_transitivity, s_modus_ponens, s_adjunction_rule]
-  >- metis_tac [s_conjunction_r, s_conjunction_l, s_transitivity, s_modus_ponens, s_adjunction_rule]
-  >- metis_tac [s_conjunction_r, s_conjunction_l, s_transitivity, s_modus_ponens, s_adjunction_rule]
-  >- metis_tac [s_conjunction_r, s_conjunction_l, s_transitivity, s_modus_ponens, s_adjunction_rule]
-  >- (strip_tac >> assume_tac s_disjunction_elim >>
-      last_x_assum $ qspecl_then [‘A’, ‘C’, ‘B Vₛ C’] strip_assume_tac >>
-      ‘slaney_provable (((A -->ₛ B Vₛ C) &ₛ C -->ₛ B Vₛ C))’ suffices_by
-        metis_tac[slaney_provable_rules]
-      >> irule s_adjunction_rule >> strip_tac
-      >- (irule s_modus_ponens >> qexists_tac ‘(B -->ₛ B Vₛ C)’ >> strip_tac
-          >- simp[s_disjunction_l]
-          >- metis_tac [s_conjunction_r, s_conjunction_l, s_transitivity,
-                        s_modus_ponens, s_adjunction_rule]
-         )
-      >- metis_tac[slaney_provable_rules]
+  rpt strip_tac >> gs[s_DIMP_def]
+  >- metis_tac[slaney_provable_rules] 
+  >- metis_tac [s_conjunction_r, s_conjunction_l, s_transitivity, s_modus_ponens, s_adjunction_rule, s_permutation, s_adjunction_rule]
+  >- metis_tac[s_transitivity, s_modus_ponens, s_conjunction_r, s_conjunction_l, s_double_negation, s_contrapositive, s_adjunction_rule]
+  >- metis_tac [s_conj_introduction, s_conjunction_r, s_conjunction_l, s_transitivity, s_modus_ponens, s_adjunction_rule, s_permutation, s_adjunction_rule]                          
+  >- metis_tac [s_conj_introduction, s_conjunction_r, s_conjunction_l, s_transitivity, s_modus_ponens, s_adjunction_rule, s_permutation, s_adjunction_rule]                          
+  >- metis_tac [s_conjunction_r, s_conjunction_l, s_transitivity, s_modus_ponens, s_adjunction_rule,
+                s_adjunction_rule, s_disjunction_elim, s_disjunction_l, s_disjunction_r]
+  >- metis_tac [s_conjunction_r, s_conjunction_l, s_transitivity, s_modus_ponens, s_adjunction_rule,
+                s_adjunction_rule, s_disjunction_elim, s_disjunction_l, s_disjunction_r]
+  >- metis_tac [s_conjunction_r, s_conjunction_l, s_transitivity, s_permutation, s_modus_ponens, s_adjunction_rule,
+                s_adjunction_rule, s_intensional_conj_lr, s_intensional_conj_rl, s_identity]
+  >- metis_tac [s_conjunction_r, s_conjunction_l, s_transitivity, s_permutation, s_modus_ponens, s_adjunction_rule,
+                s_adjunction_rule, s_intensional_conj_lr, s_intensional_conj_rl, s_identity]
+  >- (irule s_adjunction_rule >> rw[] >> irule s_conj_intro_rule >>
+      metis_tac [s_conj_introduction, s_conjunction_r, s_conjunction_l, s_transitivity, s_modus_ponens, s_adjunction_rule, s_permutation, s_adjunction_rule]                          
      )
-  >- (strip_tac >> assume_tac s_disjunction_elim >>
-      last_x_assum $ qspecl_then [‘B’, ‘C’, ‘A Vₛ C’] strip_assume_tac >>
-      ‘slaney_provable (((B -->ₛ A Vₛ C) &ₛ C -->ₛ A Vₛ C))’ suffices_by
-        metis_tac[slaney_provable_rules]
-      >> irule s_adjunction_rule >> strip_tac
-      >- (irule s_modus_ponens >> qexists_tac ‘(A -->ₛ A Vₛ C)’ >> strip_tac
-          >- simp[s_disjunction_l]
-          >- metis_tac [s_conjunction_r, s_conjunction_l, s_transitivity,
-                        s_modus_ponens, s_adjunction_rule]
-         )
-      >- metis_tac[slaney_provable_rules]
+  >- (irule s_adjunction_rule >> rw[] >> irule s_conj_intro_rule >>
+      metis_tac [s_conj_introduction, s_conjunction_r, s_conjunction_l, s_transitivity, s_modus_ponens, s_adjunction_rule, s_permutation, s_adjunction_rule]                          
      )
-  >- metis_tac[slaney_provable_rules]
   >- metis_tac[slaney_provable_rules]
 QED
 
@@ -172,32 +173,6 @@ Proof
       gs [s_DIMP_def] >> metis_tac[s_transitivity, s_conjunction_r, s_modus_ponens]
       )
 QED
-        
-Theorem s_equiv_stronger_replacement:
-  ∀A B C. slaney_provable (A <->ₛ B) ⇒
-          slaney_provable ((A -->ₛ C) <->ₛ (B -->ₛ C)) ∧
-          slaney_provable ((C -->ₛ A) <->ₛ (C -->ₛ B)) ∧
-          slaney_provable ((A &ₛ C) <->ₛ (B &ₛ C)) ∧
-          slaney_provable ((C &ₛ A) <->ₛ (C &ₛ B)) ∧
-          slaney_provable ((A Vₛ C) <->ₛ (B Vₛ C)) ∧
-          slaney_provable ((C Vₛ A) <->ₛ (C Vₛ B)) ∧
-          slaney_provable ((~ₛ A) <->ₛ (~ₛ B)) ∧
-          slaney_provable ((A ioₛ C) <->ₛ (B ioₛ C)) ∧
-          slaney_provable ((C ioₛ A) <->ₛ (C ioₛ A))
-Proof
-  rpt strip_tac >> gs[s_DIMP_def] >> irule s_adjunction_rule
-  >- metis_tac [s_modus_ponens, s_conjunction_l, s_conjunction_r, s_transitivity, s_permutation]
-  >- metis_tac [s_modus_ponens, s_conjunction_l, s_conjunction_r, s_prefixing, s_permutation]
-  >- metis_tac [s_conj_introduction, s_transitivity, s_conjunction_r, s_conjunction_l, s_adjunction_rule, s_modus_ponens]
-  >- metis_tac [s_conj_introduction, s_transitivity, s_conjunction_r, s_conjunction_l, s_adjunction_rule, s_modus_ponens]
-  >- metis_tac[s_disjunction_elim, s_disjunction_l, s_disjunction_r, s_transitivity, s_adjunction_rule, s_conjunction_l, s_conjunction_r, s_modus_ponens] 
-  >- metis_tac[s_disjunction_elim, s_disjunction_l, s_disjunction_r, s_transitivity, s_adjunction_rule, s_conjunction_l, s_conjunction_r, s_modus_ponens]
-  >- (assume_tac s_contrapositive_2 >> last_assum $ qspecl_then [‘A’, ‘B’] strip_assume_tac >>
-      last_x_assum $ qspecl_then [‘B’, ‘A’] strip_assume_tac >> 
-      metis_tac[slaney_provable_rules, s_DIMP_def]
-      )
-  >> metis_tac[s_modus_ponens, s_identity, s_conjunction_r, s_conjunction_l,  s_intensional_conj_rl,  s_intensional_conj_lr, s_transitivity]
-QED
 
 Theorem s_double_dimp_equiv:
   ∀A B C D. slaney_provable (A <->ₛ B) ∧ slaney_provable (C <->ₛ D) ⇒
@@ -213,13 +188,11 @@ Proof
   >- metis_tac[s_modus_ponens, s_identity, s_conjunction_r, s_conjunction_l,  s_intensional_conj_rl,  s_intensional_conj_lr, s_transitivity]
 QED
 
-
-        
 Theorem s_OR_definable:
   ∀A B. slaney_provable ((A Vₛ B) <->ₛ (~ₛ (~ₛ A &ₛ ~ₛ B)))
 Proof
   rw[s_DIMP_def] >> irule s_adjunction_rule >> rw[]
-  >- (irule s_modus_ponens >> qexists_tac ‘((A -->ₛ ~ₛ (~ₛ A &ₛ ~ₛ B)) &ₛ B -->ₛ ~ₛ (~ₛ A &ₛ ~ₛ B))’ >> 
+  >- (irule s_modus_ponens >> qexists_tac ‘((A -->ₛ ~ₛ (~ₛ A &ₛ ~ₛ B)) &ₛ (B -->ₛ ~ₛ (~ₛ A &ₛ ~ₛ B)))’ >> 
       assume_tac s_disjunction_elim >>
       last_x_assum $ qspecl_then [‘A’, ‘B’, ‘~ₛ (~ₛ A &ₛ ~ₛ B)’] strip_assume_tac >> rw[] >>
       irule s_adjunction_rule >>  metis_tac[slaney_provable_rules])
@@ -231,7 +204,7 @@ Proof
         metis_tac [s_double_negative_equiv, s_equiv_replacement] >>
       assume_tac s_conj_introduction >>
       last_x_assum $ qspecl_then [‘~ₛ (A Vₛ B)’, ‘~ₛ A’, ‘~ₛ B’] strip_assume_tac >>
-      ‘slaney_provable (((~ₛ (A Vₛ B) -->ₛ ~ₛ A) &ₛ ~ₛ (A Vₛ B) -->ₛ ~ₛ B))’ suffices_by
+      ‘slaney_provable (((~ₛ (A Vₛ B) -->ₛ ~ₛ A) &ₛ (~ₛ (A Vₛ B) -->ₛ ~ₛ B)))’ suffices_by
         metis_tac[s_modus_ponens] >>
       metis_tac[slaney_provable_rules, s_double_negative_equiv, s_equiv_replacement])
 QED
@@ -242,7 +215,7 @@ Proof
   rw[s_DIMP_def] >> irule s_adjunction_rule >> rw[]
   >-(irule s_intensional_conj_rl >>
      metis_tac[s_assertion, s_contrapositive, s_transitivity, s_modus_ponens])
-  >- (‘slaney_provable(A -->ₛ B -->ₛ A ioₛ B)’ by metis_tac [slaney_provable_rules] >>
+  >- (‘slaney_provable (A -->ₛ B -->ₛ (A ioₛ B))’ by metis_tac [slaney_provable_rules] >>
       metis_tac[s_contrapositive, s_contrapositive_2, s_equiv_replacement, s_permutation, s_modus_ponens])
 QED
 
