Thesis/prettyPrintingNDScript.sml
@@ -10,4 +10,11 @@ val _ = add_rule {block_style = (AroundEachPhrase, (PP.CONSISTENT, 0)),
 			term_name = "==>",
 			pp_elements = [HardSpace 1, TOK "⇒", BreakSpace(1,10)]}
 
+val _ = add_rule {block_style = (AroundEachPhrase, (PP.CONSISTENT, 0)),
+			paren_style = OnlyIfNecessary,
+			fixity = Suffix 2100,
+			term_name = "REPLACE",
+			pp_elements = [TOK "(REPLACE1)", TM, TOK "(REPLACE2)"]}
+
+
 val _ = export_theory()
